Remove [static_blit_under] and [blit_underN].
Instead, [blit] just uses [simple_blit] to deal with the case where [_n] is small.

src/array.v
@@ -1118,85 +1118,6 @@ Proof.
   wp_op wp_static_blit shadowing: b.
 Qed.
 
-(* [static_blit_under] handles all sizes [_n] comprised in the semi-open
-   interval [lo, lo+delta). The parameters [lo] and [delta] have type
-   [nat]; they exist at compile time only. *)
-
-(* TODO this logic is largely independent of [static_blit] and
-   could be generalized *)
-
-Section BU.
-Local Opaque Nat.div. (* This prevents unfolding and helps [lia]. *)
-
-Equations static_blit_under a _i b _j _n (lo delta : nat) : array A
-by wf delta lt :=
-static_blit_under a _i b _j _n lo delta :=
-  IF (delta <=? 1)%nat THEN
-    static_blit a _i b _j lo 0
-  ELSE
-    let half := (delta / 2)%nat in
-    let midpoint := (lo + half)%nat in
-    if (_n <? of_nat midpoint)%uint63 then
-      static_blit_under a _i b _j _n lo half
-    else
-      static_blit_under a _i b _j _n midpoint (delta - half).
-
-End BU.
-
-(* [static_blit_under] is correct. *)
-
-Lemma wp_static_blit_under delta :
-  ∀ lo,
-  ∀IntU _n n,
-  (lo ≤ Z.to_nat n < lo + delta)%nat →
-  unsigned (Z.of_nat (lo + delta)) →
-  blit_spec (λ a _i b _j, static_blit_under a _i b _j _n lo delta) n.
-Proof.
-  by well-founded induction on delta along lt.
-  unfold blit_spec. intros.
-  autorewrite with static_blit_under.
-  destruct (delta <=? 1)%nat eqn:Heq.
-  (* Case [delta ≤ 1]. In fact, [delta] cannot be zero, as [n] lies
-     within the semi-open interval of [lo] to [lo + delta]. So, we
-     must in fact have [delta = 1]. *)
-  { wp_op wp_static_blit shadowing: b.
-    isArray. }
-  (* Case [1 < delta]. *)
-  { wp_if; eapply IH; tc. }
-Qed.
-
-(* We can now specialize [static_blit_under] for the size [N]. *)
-
-(* This scheme generates code of quadratic size, because each size [k] up
-   to the limit [N] requires a code fragment of size [k]. If we could use
-   Duff's device then we could generate code of linear size. That would
-   require the ability to programmatically generate named (toplevel)
-   functions and function calls. *)
-
-Transparent static_blit_under.
-Definition blit_underN a _i b _j _n :=
-  Eval compute -[bind] in static_blit_under a _i b _j _n 0 N.
-
-(* Disable Notation "t .[ i ]" := (get t i). *)
-(* Disable Notation "t .[ i <- a ]" := (set t i a). *)
-(* Print blit_underN. *)
-
-(* [blit_underN] is correct. It handles all sizes less than [N]. *)
-
-Lemma wp_blit_underN :
-  ∀Int _n n,
-  (0 ≤ n < NZ)%Z →
-  blit_spec (λ a _i b _j, blit_underN a _i b _j _n) n.
-Proof.
-  unfold NZ.
-  intros.
-  unfold blit_spec. intros.
-  change (blit_underN a _i b _j _n)
-    with (static_blit_under a _i b _j _n 0 N).
-  unfold N.
-  eapply wp_static_blit_under; tc.
-Qed.
-
 (* A couple technical lemmas. *)
 
 Lemma ilt_n_minus_N {_n} :
@@ -1214,7 +1135,7 @@ Open Scope uint63.
 
 Fixpoint blit_aux a _i b _j _n (ACC : Acc ilt _n) :=
   IFC _n <? Ni THEN
-    λ _, blit_underN a _i b _j _n
+    λ _, simple_blit a _i b _j _n
   ELSE
     λ (Hlt : (_n <? Ni) = false),
     do b ← blitN a _i b _j ;
@@ -1230,7 +1151,7 @@ Lemma blit_aux_eq _n :
   ∀ a _i b _j ACC,
   blit_aux a _i b _j _n ACC =
   if _n <? Ni then
-    blit_underN a _i b _j _n
+    simple_blit a _i b _j _n
   else
     do b ← blitN a _i b _j ;
     blit a (_i + Ni) b (_j + Ni) (_n - Ni).
@@ -1254,7 +1175,7 @@ Proof.
   rewrite blit_aux_eq.
   wp_if.
   (* Base case. *)
-  { wp_op wp_blit_underN shadowing: b. }
+  { wp_op wp_simple_blit shadowing: b. }
   (* Step case. *)
   { unfold Ni.
     wp_op wp_blitN; unfold NZ; tc; last wp_shadow b.
