attic/blit_under.v
@@ -1,0 +1,78 @@
+(* [static_blit_under] handles all sizes [_n] comprised in the semi-open
+   interval [lo, lo+delta). The parameters [lo] and [delta] have type
+   [nat]; they exist at compile time only. *)
+
+(* This logic is largely independent of [static_blit] and could be
+   generalized. *)
+
+Section BU.
+Local Opaque Nat.div. (* This prevents unfolding and helps [lia]. *)
+
+Equations static_blit_under a _i b _j _n (lo delta : nat) : array A
+by wf delta lt :=
+static_blit_under a _i b _j _n lo delta :=
+  IF (delta <=? 1)%nat THEN
+    static_blit a _i b _j lo 0
+  ELSE
+    let half := (delta / 2)%nat in
+    let midpoint := (lo + half)%nat in
+    if (_n <? of_nat midpoint)%uint63 then
+      static_blit_under a _i b _j _n lo half
+    else
+      static_blit_under a _i b _j _n midpoint (delta - half).
+
+End BU.
+
+(* [static_blit_under] is correct. *)
+
+Lemma wp_static_blit_under delta :
+  ∀ lo,
+  ∀IntU _n n,
+  (lo ≤ Z.to_nat n < lo + delta)%nat →
+  unsigned (Z.of_nat (lo + delta)) →
+  blit_spec (λ a _i b _j, static_blit_under a _i b _j _n lo delta) n.
+Proof.
+  by well-founded induction on delta along lt.
+  unfold blit_spec. intros.
+  autorewrite with static_blit_under.
+  destruct (delta <=? 1)%nat eqn:Heq.
+  (* Case [delta ≤ 1]. In fact, [delta] cannot be zero, as [n] lies
+     within the semi-open interval of [lo] to [lo + delta]. So, we
+     must in fact have [delta = 1]. *)
+  { wp_op wp_static_blit shadowing: b.
+    isArray. }
+  (* Case [1 < delta]. *)
+  { wp_if; eapply IH; tc. }
+Qed.
+
+(* We can now specialize [static_blit_under] for the size [N]. *)
+
+(* This scheme generates code of quadratic size, because each size [k] up
+   to the limit [N] requires a code fragment of size [k]. If we could use
+   Duff's device then we could generate code of linear size. That would
+   require the ability to programmatically generate named (toplevel)
+   functions and function calls. *)
+
+Transparent static_blit_under.
+Definition blit_underN a _i b _j _n :=
+  Eval compute -[bind] in static_blit_under a _i b _j _n 0 N.
+
+(* Disable Notation "t .[ i ]" := (get t i). *)
+(* Disable Notation "t .[ i <- a ]" := (set t i a). *)
+(* Print blit_underN. *)
+
+(* [blit_underN] is correct. It handles all sizes less than [N]. *)
+
+Lemma wp_blit_underN :
+  ∀Int _n n,
+  (0 ≤ n < NZ)%Z →
+  blit_spec (λ a _i b _j, blit_underN a _i b _j _n) n.
+Proof.
+  unfold NZ.
+  intros.
+  unfold blit_spec. intros.
+  change (blit_underN a _i b _j _n)
+    with (static_blit_under a _i b _j _n 0 N).
+  unfold N.
+  eapply wp_static_blit_under; tc.
+Qed.
